Test server for 1.2

src/tls/test/test_server.ml
@@ -1,0 +1,7 @@
+(* Main driver for interop tests *)
+
+let _ =
+  if (Array.length Sys.argv <> 3) then
+     print_string "Usage: ./server.out <binding> <port>\n"
+  else 
+     TestServer.main Sys.argv.(1) (int_of_string Sys.argv.(2))
